src/Bedrock/End2End/X25519/GarageDoorTop.v
@@ -165,23 +165,29 @@ Lemma compiler_emitted_valid_instructions :
   bverify.bvalidInstructions Decode.RV32IM garagedoor_insns = true.
 Proof. vm_cast_no_check (eq_refl true). Qed.
 
-Definition good_transitions (s : state)(t : Semantics.trace)(s' : state) :=
-  exists ioh, SPI.mmio_trace_abstraction_relation ioh t /\
-              (BootSeq +++ stateful garagedoor_iteration s s') ioh.
-Definition good_trace t := exists s0 s, good_transitions s0 t s.
+Import SPI riscv.Platform.RiscvMachine.
+Definition only_mmio_satisfying P t :=
+  exists mmios, mmio_trace_abstraction_relation mmios t /\ P mmios.
+
+Local Notation labeled_transitions := stateful.
+Local Notation boot_seq := BootSeq.
+
+Definition protocol_invariant (s s' : state) (trace : list RiscvMachine.LogItem) :=
+  only_mmio_satisfying (boot_seq +++ labeled_transitions protocol_step s s') trace.
+Definition protocol_spec t := exists s s', protocol_invariant s s' t.
 
 Import ExprImpEventLoopSpec.
 Definition garagedoor_spec : ProgramSpec := {|
   datamem_start := MemoryLayout.heap_start ml;
   datamem_pastend := MemoryLayout.heap_pastend ml;
-  goodTrace := good_trace;
-  isReady t m := exists s0 s, good_transitions s0 t s /\ exists bs R, memrep bs R s m |}.
+  goodTrace := protocol_spec;
+  isReady t m := exists s s', protocol_invariant s' s t /\ exists bs R, memrep bs R s m |}.
 
 Lemma good_trace_from_isRead a a0 : isReady garagedoor_spec a a0 ->
   isReady garagedoor_spec a a0 /\
   ExprImpEventLoopSpec.goodTrace garagedoor_spec a.
 Proof.
-  cbv [isReady goodTrace garagedoor_spec good_trace]; intuition eauto.
+  cbv [isReady goodTrace garagedoor_spec protocol_spec]; intuition eauto.
   case H as (?&?&?&?&?&H); eauto.
 Qed.
 
@@ -214,10 +220,10 @@ Implicit Types mach : RiscvMachine.
 Local Coercion word.unsigned : word.rep >-> Z.
 
 Definition initial_conditions mach :=
-  mach.(getPc) = code_start ml /\
+  0x20400000 = mach.(getPc) /\
+  [] = mach.(getLog) /\
   mach.(getNextPc) = word.add mach.(getPc) (word.of_Z 4) /\
   regs_initialized (getRegs mach) /\
-  mach.(getLog) = [] /\
   (forall a : word32, code_start ml <= a < code_pastend ml -> In a (getXAddrs mach)) /\
   valid_machine mach /\
   (imem (code_start ml) (code_pastend ml) garagedoor_insns ⋆
@@ -233,7 +239,7 @@ Proof.
   eexists garagedoor_insns.
   eexists garagedoor_finfo.
   eexists garagedoor_stack_size.
-  rewrite garagedoor_compiler_result_ok; ssplit; trivial using compiler_emitted_valid_instructions.
+  rewrite garagedoor_compiler_result_ok; ssplit; trivial using compiler_emitted_valid_instructions; try congruence.
   2,3:vm_compute; inversion 1.
   econstructor (* ProgramSatisfiesSpec *).
   1: vm_compute; reflexivity.
@@ -241,6 +247,7 @@ Proof.
   3: instantiate (1:=snd loop).
   1,3: exact eq_refl.
   1,2: cbv [hl_inv]; intros; eapply MetricSemantics.of_metrics_free; eapply WeakestPreconditionProperties.sound_cmd.
+  3: { eapply word.unsigned_inj. rewrite <-H. trivial. }
 
   all : repeat straightline; subst args.
   { cbv [LowerPipeline.mem_available LowerPipeline.ptsto_bytes] in *.
@@ -266,7 +273,8 @@ Proof.
     rewrite <-(List.firstn_skipn 1520 (skipn 32 (skipn 64 anybytes))) in M.
     do 2 seprewrite_in @Array.bytearray_append M.
     rewrite ?firstn_length, ?skipn_length, ?Nat2Z.inj_min, ?Nat2Z.inj_sub, H6_emp0 in M.
-    cbv [isReady garagedoor_spec good_trace good_transitions]. eexists (_,_), (_,_); fwd. eauto.
+    cbv [isReady garagedoor_spec protocol_spec protocol_invariant only_mmio_satisfying].
+    eexists (Build_state _ _), (Build_state _ _); fwd. eauto.
     { rewrite <-app_nil_l. eapply TracePredicate.concat_app; eauto. econstructor. }
     cbv [memrep]. ssplit.
     { use_sep_assumption. cancel.
@@ -277,13 +285,13 @@ Proof.
     all : repeat rewrite ?firstn_length, ?skipn_length; try Lia.lia. }
 
   {  match goal with H : goodTrace _ _ |- _ => clear H end.
-    cbv [isReady goodTrace good_trace garagedoor_spec] in *; repeat straightline.
+    cbv [isReady goodTrace protocol_spec protocol_invariant garagedoor_spec] in *; repeat straightline.
     DestructHead.destruct_head' state.
     Tactics.rapply WeakestPreconditionProperties.Proper_call;
       [|eapply link_loopfn]; try eassumption.
     intros ? ? ? ?; repeat straightline; eapply good_trace_from_isRead.
     eexists; fwd; try eassumption.
-    cbv [good_trace good_transitions] in *; repeat straightline.
+    cbv [protocol_spec protocol_invariant only_mmio_satisfying] in *; repeat straightline.
     { subst a.  (eexists; split; [eapply Forall2_app; eauto|]).
       eapply stateful_app_r, stateful_singleton; eauto. } }
 Qed.
@@ -291,7 +299,7 @@ Qed.
 Theorem garagedoor_invariant_proof: exists invariant: RiscvMachine -> Prop,
    (forall mach, initial_conditions mach -> invariant mach) /\
    (forall mach, invariant mach -> run1 mach invariant) /\
-   (forall mach, invariant mach -> exists extend, good_trace (getLog mach ;++ extend)).
+   (forall mach, invariant mach -> exists extend, protocol_spec (getLog mach ;++ extend)).
 Proof.
   exists (ll_inv compile_ext_call ml garagedoor_spec).
   unshelve epose proof compiler_invariant_proofs _ _ _ _ _ garagedoor_spec as HCI; shelve_unifiable; try exact _.
@@ -305,10 +313,10 @@ Qed.
 
 Import OmniSmallstepCombinators.
 
-Theorem garagedoor_correct mach : initial_conditions mach ->
-  always run1 (eventually run1 (fun mach' => good_trace mach'.(getLog))) mach.
+Theorem garagedoor_correct : forall mach, initial_conditions mach ->
+  always run1 (eventually run1 (fun mach' => protocol_spec mach'.(getLog))) mach.
 Proof.
-  intros H%initial_conditions_sufficient; revert H.
+  intros ? H%initial_conditions_sufficient; revert H.
   unshelve Tactics.rapply @always_eventually_good_trace; trivial using ml_ok, @Naive.word32_ok.
   { eapply (naive_word_riscv_ok 5%nat). }
   { eapply @SortedListString.ok. }
